README.md
@@ -1,15 +1,15 @@
 TODO:
 
 For Plus:
-- ~~is (Literal 0) neutral on the left?~~
-- ~~is (Literal 0) neutral on the right?~~
-- ~~is Plus associative?~~
-- ~~is Plus commutative?~~
+- ~~is (Literal 0) neutral on the left? (Report)~~
+- ~~is (Literal 0) neutral on the right? (Report)~~
+- ~~is Plus associative?~~ (Report)
+- ~~is Plus commutative?~~ (Report)
 
-~~If one of these properties doesn't hold, can you state a conditional property that holds?~~
+~~If one of these properties doesn't hold, can you state a conditional property that holds?~~ (Report)
 
 For Times:
-- Implement Times
+- ~~Implement Times~~ (Report)
 - is (Literal 1) neutral on the left?
 - is (Literal 1) neutral on the right?
 - is (Literal 0) absorbing on the left?
